proved a lower bound on time gap between ev2 and ev3

icreate.v
@@ -2001,6 +2001,60 @@ Proof.
   ring.
 Qed.
 
+Definition Ev23TimeGapLB : IR :=
+  ((CRasIR ((|targetPos|)) - QposAsQ distPrec) * (Qinv speed))
+  - E2EDelVar.
+
+Lemma QDivQopp : ∀ (a b: Q),
+  (-(a /b )== ((-a )/ b))%Q.
+Proof.
+  intros.
+  destruct (decide (b=0)) as [Hd|Hd].
+- rewrite Hd. destruct a.
+  unfoldMC. unfold Qdiv, Qinv. simpl.
+  ring.
+- field. assumption.
+Qed.
+
+
+Lemma MotorEv23GapLB :
+  let t2 : QTime := MotorEventsNthTime 2 (decAuto (2<4)%nat I) in
+  let t3 : QTime := MotorEventsNthTime 3 (decAuto (3<4)%nat I) in
+   Ev23TimeGapLB  ≤  Q2R (t3 - t2).
+Proof.
+  intros ? ?.
+  pose proof MotorEv23Gap2_2 as Hp.
+  fold t2 t3 in Hp.
+  Local Opaque Q2R.
+  simpl in Hp.
+  apply AbsIR_imp_AbsSmall in Hp.
+  unfold AbsSmall in Hp.
+  apply proj1 in Hp.
+  apply shift_plus_leEq in Hp.
+  unfold Ev23TimeGapLB.
+  eapply leEq_transitive;[|apply Hp].
+  clear Hp.
+  unfold E2EDelVar.
+  unfoldMC.
+  autounfold with IRMC.
+  unfold Mult_instance_IR.
+  rewrite ring_distl_unfolded.
+  simpl.  destruct sendTimeAcc, delivDelayVar.
+  simpl. apply eqImpliesLeEq.
+  simpl.  
+  autorewrite with QSimpl. simpl.
+  Local Transparent Q2R.
+  unfold Q2R. 
+  rewrite inj_Q_inv.
+  rewrite inj_Q_inv.
+  pose proof QDivQopp as Hq.
+  unfold Qdiv in Hq.
+  rewrite <- Hq.
+  rewrite inj_Q_inv.
+  rewrite inj_Q_plus.
+  ring.
+Qed.
+
 
 Lemma ThetaEv2To3_2 :
   let t3 : QTime := MotorEventsNthTime 3 (decAuto (3<4)%nat I) in
@@ -2526,6 +2580,7 @@ Qed.
 Lemma XChangeUBEv2To3_2 :
   let t3 : QTime := MotorEventsNthTime 3 (decAuto (3<4)%nat I) in
   let t2 : QTime := MotorEventsNthTime 2 (decAuto (2<4)%nat I) in
+
    ({X rotOrigininPos} t3 [-] {X rotOrigininPos} t2) 
       ≤  (Ev23TimeGapUB * (speed + transErrTrans)%Q).
 Proof.
